\chapter{Limits}
\hi{The Squeeze theorem}
    \begin{equation}
        \begin{cases}
            f(x) \leq g(x) \leq h(x) \\
            \lim_{x \to a} f(x) = \lim_{x \to a} h(x) = L
        \end{cases}
        \Then \lim_{x \to a} g(x) = L
    \end{equation}

\hi{7 Indeterminate forms}
    \begin{equation}
        \dfrac{\infty}{\infty}, \dfrac{0}{0}, \infty - \infty, 0 \cdot \infty,
        1^{\infty}, \infty^{0}, 0^{0}
    \end{equation}

\hi{Exercise: L'Hospital's rule}
    \begin{enumerate}
        \item Indeterminate from: $\infty - \infty$
            Transform the expression: \\
            \begin{align*}
                f(x) - g(x) = \dfrac{\frac{1}{g(x)} - \frac{1}{f(x)}}{\frac{1}{g(x)}} - \frac{1}{f(x)}
            \end{align*}
    \end{enumerate}
