\chapter{Derivatives}

\hi{Derivatives of Trigonometric Functions}
    \hii{Secant, Cosecant}
        \begin{eqbox}
            & \sec'(x) = \sec(x)\tan(x) \\
            & \csc'(x) = -\csc(x)\cot(x)
        \end{eqbox}
        \textbf{Proof}
            \begin{align*}
                \sec'(x) = [\cos^{-1}(x)]' = -\cos^{-2}(x)[-\sin(x)] = \frac{\sin(x)}{\cos^{2}(x)} = \sec(x)\tan(x)
                \csc'(x) = [\sin^{-1}(x)]' = -\sin^{-2}(x)\cos(x) = - \frac{\cos(x)}{\sin^{2}(x)} = -\csc(x)\cot(x)
            \end{align*}
    \hii{Arcsin, Arccos, Arctan}
        \begin{align}
            \arcsin'(x)= \dfrac{1}{\sqrt{1 - x^{2}}} \\
            \arccos'(x) = - \dfrac{1}{\sqrt{1 - x^{2}}} \\
            \arctan'(x) = \dfrac{1}{1 + x^{2}} \\
            \mbox{arccot}'(x) = - \dfrac{1}{1 + x^{2}}
        \end{align}
